Mjollnir completed for the nop programming language

Mjollnir.v
@@ -1,5 +1,3 @@
-(* Our very simple language *)
-
 Require Import List.
 
 Inductive stmt : Type :=
@@ -7,7 +5,30 @@ Inductive stmt : Type :=
 
 Definition path : Type := list stmt.
 
+Definition state : Type := unit.
 
+Inductive correlation : Type :=
+  | states_eq : correlation
+  | true_c    : correlation.
 
+Inductive correlation_holds : correlation -> state -> state -> Prop :=
+  | states_eq_holds : forall st, correlation_holds states_eq st st
+  | true_c_holds    : forall st1 st2, correlation_holds true_c st1 st2.
 
+Definition step (s0:state) (stmt:stmt) : state :=
+  s0.
 
+Definition step_path s0 p := fold_left step p s0.
+
+Definition pec_check (c c':correlation) (p1 p2:path) : bool :=
+  false.
+
+Theorem pec_check_correct :
+  forall c c' p1 p2 sL sR,
+    correlation_holds c sL sR ->
+    pec_check c c' p1 p2 = true ->
+    correlation_holds c' (step_path sL p1) (step_path sR p2).
+Proof.
+  intros.
+  inversion H0.
+Qed.
